Problem 0

src/lean4/ProgDefs/SampleProbs/Problem_0.lean
@@ -13,5 +13,11 @@ Task 1: Find the bug in the current implementation of maxListV1
 and write a new implementation maxListV2 that will be correct.
 (Points: 4)
 -/
-def maxListV2 : List Int → Int :=
-  sorry
+def maxListV2 : List Int → Int
+| [] => 0
+| [x] => x
+| x::xs => max x (maxListV2 xs)
+
+#eval maxListV2 [3, 1, 4, 1, 5, 9, 2]
+#eval maxListV2 []
+#eval maxListV2 [-10, -5, -2]
