src/lean4/ProgVer/SampleProbs/Problem_0.lean
@@ -7,18 +7,20 @@ def maxList : List Int → Int := maxListV1
 #eval maxList [-4, -1, -1, -3, -4, -5]
 -- NOTE: the ^ above code will return 0, but answer is -1
 
-/--
+/-
 Specification for checking if the maximum of a list is correct.
 Task 2:
 (a) What is wrong with the current specification? It accepts an
 incorrect implementation of maxList. Write brief answer as a comment below.
 (Points: 2)
-Answer:
+Answer: The current specification only checks that the returned value is
+larger than every list element, not that it belongs to the list.
 
 (b) Give examples of incorrect implementations of maxList that satisfy the
 current specification, other than the one given in the code above.
 (Points: 2)
-Answer:
+Answer: Any implemenetation that always returns the max int value, or one that
+returns the max of the list plus one.
 
 -/
 lemma maxList_spec_v1
@@ -52,26 +54,85 @@ lemma maxList_spec_v1
   simp [maxList] at inductive_hypothesis
   simp [inductive_hypothesis]
 
-/--
+/-
 Task 3:
 (a) Write a correct specification for maxList `maxList_spec_v2`. (Points: 4)
 (b) Write a proof that maxList satisfies the specification. (Points: 8)
 (c) Justify that your specification is hack proof, in the sense that it
     does not accept an incorrect implementation of maxList? Write your answer
     as a comment below. (Points: 4)
-Answer:
+Answer: If the list is nonempty, the maximum of the list is the largest value present in the list.
+This means it must be 1. greater than or equal to all other elements, and 2. be an element of the list.
+The specification states this exactly, so any implementation that passes it must correctly return the max
+of a list.
 
 (d) In general, one might think that specifications are hack proof, and more stronger
     than tests. However, for `maxList_spec_v1`, we have seen that it is not hack proof.
     Suggests ways to write better specifications that cannot be
     hacked by incorrect implementations. Write your answer
     as a comment below. (Points: 4)
-Answer:
+Answer: One way could be to add additional properties to the proof that correct implementations should satisfy,
+like maxList(list :: maxList(list)+1) = maxList(list)+1. Another way is just manually writing test cases
+targeting edge cases, or maybe having an LLM trained to automatically generate adversarial tests (as long
+as they are manually verified). But in general, these just add layers of defense and can't formally verify anything.
 
 -/
+def maxList2 : List Int → Int := maxListV2
 lemma maxList_spec_v2
 (list : List Int)
 (h_list_nonempty : list ≠ [])
--- Change 0 = 0 to the correct specification
-: 0 = 0 := by
-sorry
+: maxListV2 list ∈ list ∧
+  ∀ x ∈ list,
+  x ≤ maxList2 list := by
+  constructor
+  -- maxList list ∈ list
+  induction list
+  contradiction
+
+  rename_i list_head list_tail inductive_hypothesis
+  by_cases list_tail = []
+  rename_i list_tail_empty
+  simp [list_tail_empty]
+  simp [maxList2, maxListV2]
+
+  rename_i list_tail_nonempty
+  simp [list_tail_nonempty] at inductive_hypothesis
+  simp [maxList2, maxListV2]
+  by_cases maxList2 (list_head :: list_tail) = list_head
+  rename_i x
+  simp [maxList2, maxListV2] at x
+  left
+  exact x
+
+  rename_i x
+  simp [maxList2, maxListV2] at x
+  right
+  rw [max_eq_right_of_lt]
+  exact inductive_hypothesis
+  exact x
+
+  -- x ≤ maxList2 list
+  intro x h_x_in_list
+  induction list
+  contradiction
+  rename_i list_hd list' inductive_hypothesis
+  by_cases list' = []
+  rename_i h_list'_empty
+  rw [h_list'_empty] at h_x_in_list
+  simp [h_list'_empty]
+  simp [maxList2, maxListV2]
+  simp at h_x_in_list
+  rw [h_x_in_list]
+  rename_i list'_nonempty
+  simp [list'_nonempty] at inductive_hypothesis
+  simp at h_x_in_list
+  cases h_x_in_list
+  rename_i h_eq_list_hd
+  simp [maxList2, maxListV2]
+  rw [h_eq_list_hd]
+  simp
+  rename_i h_x_in_list'
+  simp [h_x_in_list'] at inductive_hypothesis
+  simp [maxList2, maxListV2]
+  simp [maxList2] at inductive_hypothesis
+  simp [inductive_hypothesis]
